ResourceDependency.v
@@ -20,65 +20,65 @@ Module C := Graphs.Bipartite.Cycle.
 Ltac r_auto := repeat auto.
 Ltac apply_auto H := apply H; r_auto.
 
-(** We define a resource as a pair of phaser ids and a natural (the phase). *)
-Module RES := PairOrderedType PHID Nat_as_OT.
-Module Set_RES := FSetAVL.Make RES.
-Module Set_RES_Extra := SetUtil Set_RES.
-Module Map_RES := FMapAVL.Make RES.
-Module Map_RES_Extra := MapUtil Map_RES.
-Definition resource := RES.t.
-Definition set_resource := Set_RES.t.
+(** We define an event as a pair of phaser ids and a natural (the phase). *)
+Module EVT := PairOrderedType PHID Nat_as_OT.
+Module Set_EVT := FSetAVL.Make EVT.
+Module Set_EVT_Extra := SetUtil Set_EVT.
+Module Map_EVT := FMapAVL.Make EVT.
+Module Map_EVT_Extra := MapUtil Map_EVT.
+Definition event := EVT.t.
+Definition set_event := Set_EVT.t.
 
-(* Function [get_phaser] obtains the phaser id in the resource. *)
-Definition get_phaser (r:resource) : phid := fst r.
+(* Function [get_phaser] obtains the phaser id in the event. *)
+Definition get_phaser (e:event) : phid := fst e.
 
-(* Function [get_phase] obtains the phase number of the resource. *)
-Definition get_phase (r:resource) : nat := snd r.
+(* Function [get_phase] obtains the phase number of the event. *)
+Definition get_phase (e:event) : nat := snd e.
 
 (** Phases from the same phaser are in a precedes relation. *)
-Definition prec (r1:resource) (r2:resource) :=
+Definition prec (r1:event) (r2:event) :=
   get_phaser r1 = get_phaser r2 /\ get_phase r1 < get_phase r2.
 
 Section StateProps.
 
 Variable s:state.
 
-(** We say that a task [t] is waiting for a resource [r] 
+(** We say that a task [t] is waiting for an event [r] 
     when task [t] is executing an instruction [Await] and
     the target phaser is defined in the phaser map. *)
-Definition WaitsFor (t:tid) (r:resource) :=
+Definition WaitsFor (t:tid) (e:event) :=
   exists prg,
-  Map_TID.MapsTo t (pcons (Await (get_phaser r) (get_phase r)) prg) (get_tasks s) /\
-  Map_PHID.In (get_phaser r) (get_phasers s).
+  Map_TID.MapsTo t (pcons (Await (get_phaser e) (get_phase e)) prg) (get_tasks s) /\
+  Map_PHID.In (get_phaser e) (get_phasers s).
 
-(** A task [t] is registered in a resource [r] if [t] is registered
+(** A task [t] is registered in an event [r] if [t] is registered
     in phaser [get_phaser r] and in phase [get_phase r]; task [t] must
-    be waiting for some resource. *)
-Definition Registered (t:tid) (r:resource) :=
+    be waiting for some event. *)
+Definition Registered (t:tid) (e:event) :=
   exists ph,
-  Map_PHID.MapsTo (get_phaser r) ph (get_phasers s) /\
-  Map_TID.MapsTo t (get_phase r) ph /\ exists r', WaitsFor t r'.
+  Map_PHID.MapsTo (get_phaser e) ph (get_phasers s) /\
+  Map_TID.MapsTo t (get_phase e) ph /\ exists e', WaitsFor t e'.
 
-(** A resource [r] impedes a task [t] this task is registered in a
-   resource [r'] that precedes [r]; the impeding resource must be the target of
+(** an event [r] impedes a task [t] this task is registered in a
+   event [r'] that precedes [r]; the impeding event must be the target of
    a blocked task. *)
-Definition Impedes (r:resource) (t:tid) :=
-  (exists t', WaitsFor t' r) /\
-  (exists r', Registered t r' /\ prec r' r).
+Definition Impedes (e:event) (t:tid) :=
+  (exists t', WaitsFor t' e) /\
+  (exists e', Registered t e' /\ prec e' e).
 
 Lemma impedes_def:
-  forall r t t' r',
-  WaitsFor t' r ->
-  Registered t r' ->
-  prec r' r ->
-  Impedes r t.
+  forall e t t' e',
+  WaitsFor t' e ->
+  Registered t e' ->
+  prec e' e ->
+  Impedes e t.
 Proof.
   unfold Impedes.
   intros.
   split.
   - exists t'.
     assumption.
-  - exists r'.
+  - exists e'.
     intuition.
 Qed.
 
@@ -86,19 +86,19 @@ End StateProps.
 
 (** We now characterize a deadlocked state.
     Let [AllTasksWaitFor] be a state such that all tasks in the state
-    are waiting for a resource. *)
+    are waiting for an event. *)
 
 Definition AllTasksWaitFor s :=
-  forall t, (Map_TID.In t (get_tasks s) -> exists r, WaitsFor s t r).
+  forall t, (Map_TID.In t (get_tasks s) -> exists e, WaitsFor s t e).
 
 (** Let [AllBlockedRegistered] be a state such that any task waiting for
-    a resource, that resource is also impeding another task in the state. *)
+    an event, that event is also impeding another task in the state. *)
 
 Definition AllImpedes s :=
-  forall t r, WaitsFor s t r -> exists t', Impedes s r t'.
+  forall t e, WaitsFor s t e -> exists t', Impedes s e t'.
 
 (** A totally deadlocked state is such that all tasks are waiting for
-    resources that are impeding a tasks in the task map. *)
+    events that are impeding a tasks in the task map. *)
 
 Definition TotallyDeadlocked (s:state) :=
   AllTasksWaitFor s /\ AllImpedes s /\
@@ -118,7 +118,7 @@ Definition Deadlocked (s:state) :=
 (** A GRG is a bipartite graph that is defined
    from relations [WaitsFor] and [Impedes]. *)
 Definition GRG(s:state) := B.mk_bipartite _ _ (WaitsFor s) (Impedes s).
-(** By contracting the resources we get a WFG graph. *)
+(** By contracting the events we get a WFG graph. *)
 Notation WFG s := (B.contract_a (GRG s)).
 (** By contracting the tasks we get an SG graph. *)
 Notation SG s := (B.contract_b (GRG s)).
@@ -132,13 +132,13 @@ Notation RCycle s := (G.Cycle (SG s)).
 Notation t_walk := (list (tid * tid) % type).
 
 (** In WFG an arc from task [t1] to [t2] is read as [t1] waits for [t2].
-    In Brenner this means that there exists a resource [r] where task
-    [t1] is blocked and task [t2] has not arrived at resource [r].*)
+    In Brenner this means that there exists an event [e] where task
+    [t1] is blocked and task [t2] has not arrived at event [e].*)
 Lemma tedge_spec:
   forall s (t1 t2:tid),
   TEdge s (t1, t2) <->
-  exists r,
-  WaitsFor s t1 r /\ Impedes s r t2.
+  exists e,
+  WaitsFor s t1 e /\ Impedes s e t2.
 Proof.
   split.
   + intros.
@@ -148,24 +148,24 @@ Proof.
     exists b.
     intuition.
   + intros.
-    destruct H as (r, (H1, H2)).
+    destruct H as (e, (H1, H2)).
     simpl.
-    apply Core.aa with (b:=r); repeat auto.
+    apply Core.aa with (b:=e); repeat auto.
 Qed.
 
-(** In an SG an arc from [r1] to [r2] can be read
-    as resource [r1] happens before resource [r2].
+(** In an SG an arc from [e1] to [e2] can be read
+    as event [e1] happens before event [e2].
     In Brenner, this means that there is a task [t]
-    blocked in [r2] and impedes [r1]. Recall the definition
+    blocked in [e2] and impedes [e1]. Recall the definition
     of [Impedes] that states that [t] is registered in
-    a resource [r'] that precedes [r]; and that resource
-    [r] is obtained because there exists some task blocked
-    in [r] (again by definition). *)
+    an event [e'] that precedes [e]; and that event
+    [e] is obtained because there exists some task blocked
+    in [e] (again by definition). *)
 Lemma redge_spec:
-  forall s (r1 r2:resource),
-  REdge s (r1, r2) <->
+  forall s (e1 e2:event),
+  REdge s (e1, e2) <->
   exists t,
-  Impedes s r1 t /\ WaitsFor s t r2.
+  Impedes s e1 t /\ WaitsFor s t e2.
 Proof.
   split.
   - intros.
@@ -212,12 +212,12 @@ Section Basic.
 
 (** In our language tasks can only await a single phaser, so
     it is easy to see that the [WaitsFor] predicate is actually a function
-    from task ids to resources. *)
+    from task ids to events. *)
 Lemma waits_for_fun:
-  forall t r r',
-  WaitsFor s t r ->
-  WaitsFor s t r' ->
-  r = r'.
+  forall t e e',
+  WaitsFor s t e ->
+  WaitsFor s t e' ->
+  e = e'.
 Proof.
   intros.
   unfold WaitsFor in *.
@@ -227,16 +227,16 @@ Proof.
   assert (Heq:= @Map_TID_Facts.MapsTo_fun _ _ _ _ _
           H1 H3).
   inversion Heq.
-  destruct r as (p,n).
-  destruct r' as (p', n').
+  destruct e as (p,n).
+  destruct e' as (p', n').
   simpl in *.
   auto.
 Qed.
 
 (** We show that any task id in the [WaitsFor] is in the task map of [s]. *)
 Lemma waits_for_in_tasks:
-  forall t r,
-  WaitsFor s t r ->
+  forall t e,
+  WaitsFor s t e ->
   Map_TID.In t (get_tasks s).
 Proof.
   intros.
@@ -246,11 +246,11 @@ Proof.
   assumption.
 Qed.
 
-(** Any registered task is waiting for some resource. *)
+(** Any registered task is waiting for some event. *)
 Lemma registered_to_blocked:
-  forall t r,
-  Registered s t r ->
-  exists r', WaitsFor s t r'.
+  forall t e,
+  Registered s t e ->
+  exists e', WaitsFor s t e'.
 Proof.
   intros.
   unfold Registered in H.
@@ -259,14 +259,14 @@ Proof.
 Qed.
 
 Lemma impedes_in_tasks:
-  forall r t,
-  Impedes s r t ->
+  forall e t,
+  Impedes s e t ->
   Map_TID.In (elt:=prog) t (get_tasks s).
 Proof.
   intros.
-  destruct H as (_, (r', (H,_))).
+  destruct H as (_, (e', (H,_))).
   apply registered_to_blocked in H.
-  destruct H as (r'', Hb).
+  destruct H as (e'', Hb).
   unfold WaitsFor in Hb.
   destruct Hb as (prg, (Hmt, _)).
   apply Map_TID_Extra.mapsto_to_in in Hmt.
@@ -274,9 +274,9 @@ Proof.
 Qed.
 
 Lemma impedes_in_phasermap:
-  forall r t,
-  Impedes s r t ->
-  Map_PHID.In (elt:=Phaser.phaser) (get_phaser r) (get_phasers s).
+  forall e t,
+  Impedes s e t ->
+  Map_PHID.In (elt:=Phaser.phaser) (get_phaser e) (get_phasers s).
 Proof.
   intros.
   destruct H as ((t',H),_).
